
\documentclass{article}
\usepackage{amsfonts}

%%%%%%%%%%%%%%%%%%%%%%%%%%%%%%%%%%%%%%%%%%%%%%%%%%%%%%%%%%%%%%%%%%%%%%%%%%%%%%%%%%%%%%%%%%%%%%%%%%%%%%%%%%%%%%%%%%%%%%%%%%%%%%%%%%%%%%%%%%%%%%%%%%%%%%%%%%%%%%%%%%%%%%%%%%%%%%%%%%%%%%%%%%%%%%%%%%%%%%%%%%%%%%%%%%%%%%%%%%%%%%%%%%%
\usepackage{amsmath}
\usepackage{accents}

\setcounter{MaxMatrixCols}{10}
%TCIDATA{OutputFilter=LATEX.DLL}
%TCIDATA{Version=5.00.0.2606}
%TCIDATA{<META NAME="SaveForMode" CONTENT="1">}
%TCIDATA{BibliographyScheme=Manual}
%TCIDATA{Created=Wednesday, November 25, 2015 15:33:37}
%TCIDATA{LastRevised=Wednesday, November 25, 2015 17:07:32}
%TCIDATA{<META NAME="GraphicsSave" CONTENT="32">}
%TCIDATA{<META NAME="DocumentShell" CONTENT="Standard LaTeX\Blank - Standard LaTeX Article">}
%TCIDATA{CSTFile=40 LaTeX article.cst}

\newtheorem{theorem}{Theorem}
\newtheorem{acknowledgement}[theorem]{Acknowledgement}
\newtheorem{algorithm}[theorem]{Algorithm}
\newtheorem{axiom}[theorem]{Axiom}
\newtheorem{case}[theorem]{Case}
\newtheorem{claim}[theorem]{Claim}
\newtheorem{conclusion}[theorem]{Conclusion}
\newtheorem{condition}[theorem]{Condition}
\newtheorem{conjecture}[theorem]{Conjecture}
\newtheorem{corollary}[theorem]{Corollary}
\newtheorem{criterion}[theorem]{Criterion}
\newtheorem{definition}[theorem]{Definition}
\newtheorem{example}[theorem]{Example}
\newtheorem{exercise}[theorem]{Exercise}
\newtheorem{lemma}[theorem]{Lemma}
\newtheorem{notation}[theorem]{Notation}
\newtheorem{problem}[theorem]{Problem}
\newtheorem{proposition}[theorem]{Proposition}
\newtheorem{remark}[theorem]{Remark}
\newtheorem{solution}[theorem]{Solution}
\newtheorem{summary}[theorem]{Summary}
\newenvironment{proof}[1][Proof]{\noindent\textbf{#1.} }{\ \rule{0.5em}{0.5em}}
\input{../tcilatex}
\DeclareMathAccent{\wtilde}{\mathord}{largesymbols}{"65}

\begin{document}


\section{Minimax Estimation}

\begin{equation}
\underset{\hat{\beta}\in \mathbb{A}}{\min }\,\underset{\beta \in \mathbb{B}}{%
\sup }=\underset{\beta \in \mathbb{B}}{\sup }\left( \underaccent{\wtilde}{%
\hat{\beta}}^{\ast },\underaccent{\wtilde}{\beta},A\right) \Rightarrow \hat{%
\beta}^{\ast }\text{ is minimax}
\end{equation}

\begin{theorem}
Inequality Restrictions
\end{theorem}

Restriction on $\underaccent{\wtilde}{\beta}$: $A\underaccent{\wtilde}{\beta}%
\leq a\qquad a:$know vector(by priori knowledge)

\begin{equation}
\min \,\text{\c{S}}\left( \underaccent{\wtilde}{\beta}\right) =\left( Y-x%
\underaccent{\wtilde}{\beta}\right) ^{T}\left( Y-x\underaccent{\wtilde}{%
\beta}\right)
\end{equation}

Assume $a_{i}\leq \beta _{i}\leq b_{i}$ ($a_{i}$, $b_{i}$ known)

take%
\begin{equation}
\frac{\left\vert \beta _{i}-\frac{\left( a_{i}+b_{i}\right) }{2}\right\vert 
}{\frac{\left( b_{i}-a_{i}\right) }{2}}\leq 1\qquad \forall \quad i
\end{equation}

We want an ellipsoid $\left( \underaccent{\wtilde}{\beta}-%
\underaccent{\wtilde}{\beta}_{0}\right) ^{^{\prime }}T\left( %
\underaccent{\wtilde}{\beta}-\underaccent{\wtilde}{\beta}_{0}\right) \leq 1$%
, which encloses the and fullness the following condition:

\begin{enumerate}
\item The ellipsoid and cuboid have the same center point%
\begin{equation}
(i.e.)\quad \underaccent{\wtilde}{\beta}_{0}=\frac{1}{2}\left(
a_{1}+b_{1},\cdots ,a_{k}+b_{k}\right) ^{T}
\end{equation}

\item The axes of ellipsoid are parallel the coordiated so%
\begin{equation}
T=diag\left( t_{1},\cdots ,t_{k}\right)
\end{equation}

\item The corner points of the cuboin are on the surface of the ellipsoid%
\begin{equation}
(i.e.)\quad \dsum\limits_{i=1}^{k}\left( \frac{a_{i}-b_{i}}{2}\right)
^{2}t_{i}=1
\end{equation}

\item The dllipsoid has minimum volume%
\begin{eqnarray}
\min \,V_{k} &=&C_{k}\dprod\limits_{i=1}^{k}t_{i}^{\frac{1}{2}} \\
&&C_{k}\text{ dependent on the dimension K} \\
s.t.\qquad \dsum\limits_{i=1}^{k}\left( \frac{a_{i}-b_{i}}{2}\right)
^{2}t_{i} &=&1
\end{eqnarray}
\end{enumerate}

\bigskip

take \~{V}$_{k}=\dprod\limits_{i=1}^{k}t_{i}^{-1}-\lambda \left(
\dsum\limits_{i=1}^{k}\left( \frac{a_{i}-b_{i}}{2}\right) ^{2}t_{i}-1\right) 
$

\begin{eqnarray}
\frac{\partial \tilde{V}_{k}}{\partial t_{j}} &=&\dprod\limits_{i\neq
j}^{k}t_{j}^{-1}-\lambda \left( \frac{a_{i}-b_{i}}{2}\right) ^{2}=0 \\
\frac{\partial \tilde{V}_{k}}{\partial t_{j}} &=&\dsum\limits_{{}}^{{}}%
\left( \frac{a_{i}-b_{i}}{2}\right) ^{2}t_{i}-1=0
\end{eqnarray}

\end{document}
