
\documentclass{article}
%%%%%%%%%%%%%%%%%%%%%%%%%%%%%%%%%%%%%%%%%%%%%%%%%%%%%%%%%%%%%%%%%%%%%%%%%%%%%%%%%%%%%%%%%%%%%%%%%%%%%%%%%%%%%%%%%%%%%%%%%%%%%%%%%%%%%%%%%%%%%%%%%%%%%%%%%%%%%%%%%%%%%%%%%%%%%%%%%%%%%%%%%%%%%%%%%%%%%%%%%%%%%%%%%%%%%%%%%%%%%%%%%%%%%%%%%%%%%%%%%%%%%%%%%%%%
\usepackage{amssymb}
\usepackage{amsfonts}
\usepackage{amsmath}
\usepackage{accents}
\usepackage[ignoreall]{geometry}
\usepackage{fancyhdr}

\setcounter{MaxMatrixCols}{10}
%TCIDATA{OutputFilter=LATEX.DLL}
%TCIDATA{Version=5.00.0.2606}
%TCIDATA{<META NAME="SaveForMode" CONTENT="1">}
%TCIDATA{BibliographyScheme=Manual}
%TCIDATA{Created=Wednesday, November 25, 2015 15:33:37}
%TCIDATA{LastRevised=Friday, December 04, 2015 11:55:02}
%TCIDATA{<META NAME="GraphicsSave" CONTENT="32">}
%TCIDATA{<META NAME="DocumentShell" CONTENT="Standard LaTeX\Blank - Standard LaTeX Article">}
%TCIDATA{CSTFile=40 LaTeX article.cst}

\newtheorem{theorem}{Theorem}
\newtheorem{acknowledgement}[theorem]{Acknowledgement}
\newtheorem{algorithm}[theorem]{Algorithm}
\newtheorem{axiom}[theorem]{Axiom}
\newtheorem{case}[theorem]{Case}
\newtheorem{claim}[theorem]{Claim}
\newtheorem{conclusion}[theorem]{Conclusion}
\newtheorem{condition}[theorem]{Condition}
\newtheorem{conjecture}[theorem]{Conjecture}
\newtheorem{corollary}[theorem]{Corollary}
\newtheorem{criterion}[theorem]{Criterion}
\newtheorem{definition}[theorem]{Definition}
\newtheorem{example}[theorem]{Example}
\newtheorem{exercise}[theorem]{Exercise}
\newtheorem{lemma}[theorem]{Lemma}
\newtheorem{notation}[theorem]{Notation}
\newtheorem{problem}[theorem]{Problem}
\newtheorem{proposition}[theorem]{Proposition}
\newtheorem{remark}[theorem]{Remark}
\newtheorem{solution}[theorem]{Solution}
\newtheorem{summary}[theorem]{Summary}
\newenvironment{proof}[1][Proof]{\noindent\textbf{#1.} }{\ \rule{0.5em}{0.5em}}
\input{../tcilatex}
\DeclareMathAccent{\wtilde}{\mathord}{largesymbols}{"65}
\pagestyle{fancy}
\fancyfoot[C]{\thepage}

\input{tcilatex}

\begin{document}


\part{The Generalized Linear Regression Model}

\begin{equation*}
Y=x\beta +%
%TCIMACRO{\TeXButton{underaccent_epsilon}{\underaccent{\wtilde}{\epsilon}}}%
%BeginExpansion
\underaccent{\wtilde}{\epsilon}%
%EndExpansion
\quad E\left( 
%TCIMACRO{\TeXButton{underaccent_epsilon}{\underaccent{\wtilde}{\epsilon}}}%
%BeginExpansion
\underaccent{\wtilde}{\epsilon}%
%EndExpansion
\right) =0\quad Cov\left( 
%TCIMACRO{\TeXButton{underaccent_epsilon}{\underaccent{\wtilde}{\epsilon}}}%
%BeginExpansion
\underaccent{\wtilde}{\epsilon}%
%EndExpansion
\right) =\sigma ^{2}W,\quad W=p\cdot d\cdot m
\end{equation*}%
rank(x)=k, we want to estimate $%
%TCIMACRO{\TeXButton{underaccent_beta}{\underaccent{\wtilde}{\beta}}}%
%BeginExpansion
\underaccent{\wtilde}{\beta}%
%EndExpansion
$

W know

Consider linear in the response vector $%
%TCIMACRO{\TeXButton{underaccent_Y}{\underaccent{\wtilde}{Y}}}%
%BeginExpansion
\underaccent{\wtilde}{Y}%
%EndExpansion
,$ $\hat{\beta}=CY+%
%TCIMACRO{\TeXButton{underaccent_d}{\underaccent{\wtilde}{d}}}%
%BeginExpansion
\underaccent{\wtilde}{d}%
%EndExpansion
$%
\begin{equation*}
R_{1}\left( \tilde{\beta},\beta ,A\right) =E\left( \left( \tilde{\beta}%
-\beta \right) ^{\dagger }A\left( \tilde{\beta}-\beta \right) \right) \qquad
A=pdm
\end{equation*}%
\begin{equation*}
R_{2}\left( \tilde{\beta},\beta ,%
%TCIMACRO{\TeXButton{underaccent_a}{\underaccent{\wtilde}{a}}}%
%BeginExpansion
\underaccent{\wtilde}{a}%
%EndExpansion
%TCIMACRO{\TeXButton{underaccent_a}{\underaccent{\wtilde}{a}}}%
%BeginExpansion
\underaccent{\wtilde}{a}%
%EndExpansion
^{\dagger }\right) =E\left( \left( \tilde{\beta}-\beta \right) ^{\dagger }%
%TCIMACRO{\TeXButton{underaccent_a}{\underaccent{\wtilde}{a}}}%
%BeginExpansion
\underaccent{\wtilde}{a}%
%EndExpansion
%TCIMACRO{\TeXButton{underaccent_a}{\underaccent{\wtilde}{a}}}%
%BeginExpansion
\underaccent{\wtilde}{a}%
%EndExpansion
^{\dagger }\left( \tilde{\beta}-\beta \right) \right)
\end{equation*}%
\begin{equation*}
R_{3}\left( \tilde{\beta},\beta \right) =E\left( \left( Y-x\tilde{\beta}%
\right) ^{\dagger }W^{-1}\left( Y-x\tilde{\beta}\right) \right)
\end{equation*}

\paragraph{R$_{1}$-optional estimators}

\begin{enumerate}
\item heterogeneious case $\tilde{\beta}=CY+d$%
\begin{equation*}
\tilde{\beta}-\beta =CY+d-\beta =C\left( x\beta +\varepsilon \right)
+d-\beta =\left( Cx-I\right) \beta +d+C\varepsilon
\end{equation*}%
\begin{equation*}
R_{1}\left( 
%TCIMACRO{\TeXButton{underaccent_beta}{\underaccent{\wtilde}{\beta}}}%
%BeginExpansion
\underaccent{\wtilde}{\beta}%
%EndExpansion
,\beta ,A\right) =E\left[ \left( Cx-I\right) \beta +d+C\varepsilon \right]
^{\dagger }A\left[ \left( Cx-I\right) \beta +d+C\varepsilon \right]
\end{equation*}%
\begin{equation*}
=\left[ \left( Cx-I\right) \beta +d\right] ^{\dagger }A\left[ \left(
Cx-I\right) \beta +d\right] +E\left[ \left( C\varepsilon \right) ^{\dagger
}A\left( C\varepsilon \right) \right]
\end{equation*}%
Consider $%
%TCIMACRO{\TeXButton{underaccent_d}{\underaccent{\wtilde}{d}}}%
%BeginExpansion
\underaccent{\wtilde}{d}%
%EndExpansion
=-\left( Cx-I\right) \beta $%
\begin{eqnarray}
\min \quad R_{1}\left( 
%TCIMACRO{\TeXButton{underaccent_beta}{\underaccent{\wtilde}{\beta}}}%
%BeginExpansion
\underaccent{\wtilde}{\beta}%
%EndExpansion
,\beta ,A\right) &=&\underset{C}{\min }\quad E\left[ \left( C\varepsilon
\right) ^{\dagger }A\left( C\varepsilon \right) \right]  \notag \\
&=&\underset{C}{\min }\quad E\left[ \varepsilon ^{\dagger }C^{\dagger
}AC\varepsilon \right]  \notag \\
&&\underset{C}{=\min }\quad tr\left( ACE\left( \varepsilon ^{\dagger
}\varepsilon \right) C^{\dagger }\right)  \notag \\
&&\underset{C}{=\min }\quad tr\left\{ \sigma ^{2}ACWC^{\dagger }\right\} 
\underline{\qquad }\left( \ast \right)
\end{eqnarray}%
$\frac{\partial \left( \ast \right) }{\partial C}=0$ by Thm A.93\symbol{126}%
A.95, $\Rightarrow 2\sigma ^{2}ACW=0\quad \Rightarrow C=0,$ $\because \tilde{%
\beta}=CY+%
%TCIMACRO{\TeXButton{underaccent_d}{\underaccent{\wtilde}{d}}}%
%BeginExpansion
\underaccent{\wtilde}{d}%
%EndExpansion
,$ $C=0,$ $\tilde{\beta}=%
%TCIMACRO{\TeXButton{underaccent_d}{\underaccent{\wtilde}{d}}}%
%BeginExpansion
\underaccent{\wtilde}{d}%
%EndExpansion
\quad $usefullness$_{\#}$

\item homo case $\tilde{\beta}=CY$%
\begin{equation*}
R_{1}\left( \tilde{\beta},\beta ,A\right) =E\left[ \left( Cx-I\right) \beta %
\right] ^{\dagger }A\left[ \left( Cx-I\right) \beta \right] +tr\left\{
\sigma ^{2}ACWC^{\dagger }\right\}
\end{equation*}%
\begin{equation*}
\frac{\partial R_{1}}{\partial C}=2A\left[ C\left( x%
%TCIMACRO{\TeXButton{underaccent_beta}{\underaccent{\wtilde}{\beta}}}%
%BeginExpansion
\underaccent{\wtilde}{\beta}%
%EndExpansion
%TCIMACRO{\TeXButton{underaccent_beta}{\underaccent{\wtilde}{\beta}}}%
%BeginExpansion
\underaccent{\wtilde}{\beta}%
%EndExpansion
^{\dagger }x^{\dagger }\right) -\beta \beta ^{\dagger }x^{\dagger }\right] =0
\end{equation*}%
\begin{equation*}
\Rightarrow \tilde{C}_{2}=\beta \beta ^{\dagger }x^{\dagger }\left( x%
%TCIMACRO{\TeXButton{underaccent_beta}{\underaccent{\wtilde}{\beta}}}%
%BeginExpansion
\underaccent{\wtilde}{\beta}%
%EndExpansion
%TCIMACRO{\TeXButton{underaccent_beta}{\underaccent{\wtilde}{\beta}}}%
%BeginExpansion
\underaccent{\wtilde}{\beta}%
%EndExpansion
^{\dagger }x^{\dagger }+\sigma ^{2}W\right) ^{-1}
\end{equation*}
\end{enumerate}

\bigskip

December 1

\begin{equation*}
Y=x\beta +\varepsilon \quad Cov\left( 
%TCIMACRO{\TeXButton{underaccent_epsilon}{\underaccent{\wtilde}{\epsilon}}}%
%BeginExpansion
\underaccent{\wtilde}{\epsilon}%
%EndExpansion
\right) =W
\end{equation*}%
where W is p.d.m.%
\begin{equation*}
R_{1}\left( \tilde{\beta},\beta ,A\right) =E\left\{ \left( \tilde{\beta}%
-\beta \right) ^{\dagger }A\left( \tilde{\beta}-\beta \right) \right\}
\end{equation*}%
\begin{equation*}
\left\{ 
\begin{array}{c}
\text{heterogeneous}\text{: usefullness} \\ 
\text{homogeneous}\text{:}\tilde{\beta}=%
%TCIMACRO{\TeXButton{underaccent_beta}{\underaccent{\wtilde}{\beta}}}%
%BeginExpansion
\underaccent{\wtilde}{\beta}%
%EndExpansion
\frac{\beta ^{\dagger }xW^{-1}Y}{\sigma ^{2}+\beta ^{\dagger }\text{\c{S}}%
\beta },\text{\quad \c{S}}=x^{\dagger }W^{-1}x \\ 
\text{homogeneous}\text{: unbiased}\underline{\qquad }\left( \ast \right)%
\end{array}%
\right.
\end{equation*}%
\begin{equation*}
R_{2}\left( \tilde{\beta},\beta ,a\right) =E\left\{ a^{\dagger }\left( 
\tilde{\beta}-\beta \right) \right\} ^{2}
\end{equation*}%
\begin{equation*}
R_{3}=\left( \tilde{\beta},\beta \right) =E\left\{ \left( Y-x%
%TCIMACRO{%
%\TeXButton{underaccent_beta_hat}{\underaccent{\wtilde}{\hat{\beta}}}}%
%BeginExpansion
\underaccent{\wtilde}{\hat{\beta}}%
%EndExpansion
\right) ^{\dagger }W^{-1}\left( Y-x%
%TCIMACRO{%
%\TeXButton{underaccent_beta_hat}{\underaccent{\wtilde}{\hat{\beta}}}}%
%BeginExpansion
\underaccent{\wtilde}{\hat{\beta}}%
%EndExpansion
\right) \right\}
\end{equation*}%
$\left( \ast \right) $ let CY is a homogeneous estimator of $%
%TCIMACRO{%
%\TeXButton{underaccent_beta_hat}{\underaccent{\wtilde}{\hat{\beta}}}}%
%BeginExpansion
\underaccent{\wtilde}{\hat{\beta}}%
%EndExpansion
$ if c$%
%TCIMACRO{\TeXButton{underaccent_Y}{\underaccent{\wtilde}{Y}}}%
%BeginExpansion
\underaccent{\wtilde}{Y}%
%EndExpansion
$ is unbiased%
\begin{equation*}
E\left( CY\right) =cx\beta =\beta \quad \forall \beta \Rightarrow
Cx=I\Rightarrow C_{i}^{\dagger }x-e_{i}^{\dagger }=%
%TCIMACRO{\TeXButton{underaccent_o}{\underaccent{\wtilde}{o}}}%
%BeginExpansion
\underaccent{\wtilde}{o}%
%EndExpansion
_{i}^{\dagger }\quad i=1,\cdots ,t
\end{equation*}%
$C_{i}^{\dagger }$ and $e_{i}^{\dagger }$ are the ith rwo vector of $%
%TCIMACRO{\TeXButton{underaccent_C}{\underaccent{\wtilde}{C}}}%
%BeginExpansion
\underaccent{\wtilde}{C}%
%EndExpansion
$ and $I$.

\begin{equation*}
\tilde{R}_{1}\left( \tilde{\beta},\beta ,A\right) =\sigma ^{2}tr\left\{
ACWC^{\dagger }\right\}
\end{equation*}%
\begin{equation*}
\Rightarrow \underset{C}{\min }\quad \tilde{R}_{1}=\underset{C}{\min }\quad
\left\{ \sigma ^{2}tr\left\{ ACWC^{\dagger }\right\} \right\}
\end{equation*}%
\begin{equation*}
%TCIMACRO{\U{211a} }%
%BeginExpansion
\mathbb{Q}
%EndExpansion
=\sigma ^{2}tr\left\{ ACWC^{\dagger }\right\} -2\frac{\dsum \lambda
_{i}^{\dagger }\left( C_{i}^{\dagger }x-e_{i}^{\dagger }\right) }{\lambda
\left( Cx-I\right) }
\end{equation*}%
$\lambda _{i}$ are k-vector of Lagrogion multipliers $i=1,\cdots ,k$

Let $\Lambda ^{\dagger }=\left( \lambda _{1},\cdots ,\lambda _{k}\right) $%
\begin{equation*}
\frac{\partial 
%TCIMACRO{\U{211a} }%
%BeginExpansion
\mathbb{Q}
%EndExpansion
}{\partial C}=2\sigma ^{2}ACW-2\Lambda x^{\dagger }\Rightarrow \sigma
^{2}ACW=\Lambda x^{\dagger }
\end{equation*}%
\begin{equation*}
\Rightarrow \sigma ^{2}ACx=\Lambda x^{\dagger }W^{-1}x\Rightarrow \Lambda
=\sigma ^{2}ACx\left( x^{\dagger }W^{-1}x\right) ^{-1}
\end{equation*}

Since Cx=I $\Rightarrow \Lambda =\sigma ^{2}A\left( x^{\dagger
}W^{-1}x\right) ^{-1}$%
\begin{equation*}
\Rightarrow \sigma ^{2}AC=\underset{\Lambda }{\underbrace{\sigma ^{2}A\left(
x^{\dagger }W^{-1}x\right) ^{-1}}}x^{\dagger }W^{-1}
\end{equation*}%
\begin{equation*}
\therefore \tilde{C}_{3}=\left( x^{\dagger }W^{-1}x\right) ^{-1}x^{\dagger
}W^{-1}
\end{equation*}%
\begin{equation*}
\therefore \tilde{\beta}_{3}=\left( x^{\dagger }W^{-1}x\right)
^{-1}x^{\dagger }W^{-1}%
%TCIMACRO{\TeXButton{underaccent_Y}{\underaccent{\wtilde}{Y}}}%
%BeginExpansion
\underaccent{\wtilde}{Y}%
%EndExpansion
\quad \blacktriangle 
\end{equation*}%
\begin{eqnarray*}
\tilde{R}_{1}\left( \tilde{\beta}_{3},\beta ,A\right)  &=&\sigma
^{2}tr\left\{ A\tilde{C}_{3}W\tilde{C}_{3}^{\dagger }\right\}  \\
&=&\sigma ^{2}tr\left\{ A\left( x^{\dagger }W^{-1}x\right) ^{-1}x^{\dagger
}W^{-1}x\left( x^{\dagger }W^{-1}x\right) ^{-1}\right\}  \\
&=&\sigma ^{2}tr\left\{ A\left( x^{\dagger }W^{-1}x\right) ^{-1}\right\} 
\end{eqnarray*}%
\begin{eqnarray*}
Cov\left( \tilde{\beta}_{3}\right)  &=&\left( x^{\dagger }W^{-1}x\right)
^{-1}x^{\dagger }W^{-1}WW^{-1}x\left( x^{\dagger }W^{-1}x\right) ^{-1} \\
&=&\sigma ^{2}\left( x^{\dagger }W^{-1}x\right) ^{-1}
\end{eqnarray*}

\paragraph{R$_{2}$-optional estimator}

\begin{equation*}
R_{2}\left( \tilde{\beta},\beta ,%
%TCIMACRO{\TeXButton{underaccent_a}{\underaccent{\wtilde}{a}}}%
%BeginExpansion
\underaccent{\wtilde}{a}%
%EndExpansion
\right) =E\left[ a^{\dagger }\left( \tilde{\beta}-\beta \right) \right]
^{2}=E\left[ \left( \tilde{\beta}-\beta \right) ^{\dagger }aa^{\dagger
}\left( \tilde{\beta}-\beta \right) \right]
\end{equation*}

\begin{theorem}
The criteria R$_{1}$ and R$_{2}$ are equivalent.
\end{theorem}

\begin{proof}
$A=\tsum \lambda _{i}P_{i}P_{i}^{\dagger }$, $\left( \lambda
_{i},P_{i}\right) $ are eig-value and eig-vector paires of A
\end{proof}

First we want to show R$_{2}$-optional estimator $\hat{\beta}$ is R$_{1}$%
-optional. If $\hat{\beta}$ is R$_{2}$-optional then for any estimator $\hat{%
\beta}$ and for the choice of $%
%TCIMACRO{\TeXButton{underaccent_a}{\underaccent{\wtilde}{a}}}%
%BeginExpansion
\underaccent{\wtilde}{a}%
%EndExpansion
=\sqrt{\lambda _{i}}P_{i}\quad i=1,\cdots ,k$%
\begin{equation*}
\lambda _{i}E\left\{ \left( \hat{\beta}-\beta \right) ^{\dagger
}P_{i}P_{i}^{\dagger }\left( \hat{\beta}-\beta \right) \right\} \leq \lambda
_{i}E\left\{ \left( \tilde{\beta}-\beta \right) ^{\dagger
}P_{i}P_{i}^{\dagger }\left( \tilde{\beta}-\beta \right) \right\}
\end{equation*}%
$\hat{\beta}$ is R$_{2}$-optional%
\begin{equation*}
\Rightarrow E\left\{ \left( \hat{\beta}-\beta \right) ^{\dagger }\dsum
\lambda _{i}P_{i}P_{i}^{\dagger }\left( \hat{\beta}-\beta \right) \right\}
\leq E\left\{ \left( \tilde{\beta}-\beta \right) ^{\dagger }\dsum \lambda
_{i}P_{i}P_{i}^{\dagger }\left( \tilde{\beta}-\beta \right) \right\}
\end{equation*}%
\begin{equation*}
\Rightarrow E\left\{ \left( \hat{\beta}-\beta \right) ^{\dagger }A\left( 
\hat{\beta}-\beta \right) \right\} \leq E\left\{ \left( \tilde{\beta}-\beta
\right) ^{\dagger }A\left( \tilde{\beta}-\beta \right) \right\}
\end{equation*}

\end{document}
