
\documentclass{article}
%%%%%%%%%%%%%%%%%%%%%%%%%%%%%%%%%%%%%%%%%%%%%%%%%%%%%%%%%%%%%%%%%%%%%%%%%%%%%%%%%%%%%%%%%%%%%%%%%%%%%%%%%%%%%%%%%%%%%%%%%%%%%%%%%%%%%%%%%%%%%%%%%%%%%%%%%%%%%%%%%%%%%%%%%%%%%%%%%%%%%%%%%%%%%%%%%%%%%%%%%%%%%%%%%%%%%%%%%%%%%%%%%%%%%%%%%%%%%%%%%%%%%%%%%%%%
\usepackage{amssymb}
\usepackage{amsfonts}
\usepackage{amsmath}
\usepackage{accents}
\usepackage[ignoreall,a4paper]{geometry}
\usepackage{fancyhdr}

\setcounter{MaxMatrixCols}{10}
%TCIDATA{OutputFilter=LATEX.DLL}
%TCIDATA{Version=5.00.0.2606}
%TCIDATA{<META NAME="SaveForMode" CONTENT="1">}
%TCIDATA{BibliographyScheme=Manual}
%TCIDATA{Created=Wednesday, November 25, 2015 15:33:37}
%TCIDATA{LastRevised=Monday, July 11, 2016 17:18:15}
%TCIDATA{<META NAME="GraphicsSave" CONTENT="32">}
%TCIDATA{<META NAME="DocumentShell" CONTENT="Standard LaTeX\Blank - Standard LaTeX Article">}
%TCIDATA{CSTFile=40 LaTeX article.cst}
%TCIDATA{ComputeDefs=
%$W=\left( 1-\sigma \right) I$
%}


\newtheorem{theorem}{Theorem}
\newtheorem{acknowledgement}[theorem]{Acknowledgement}
\newtheorem{algorithm}[theorem]{Algorithm}
\newtheorem{axiom}[theorem]{Axiom}
\newtheorem{case}[theorem]{Case}
\newtheorem{claim}[theorem]{Claim}
\newtheorem{conclusion}[theorem]{Conclusion}
\newtheorem{condition}[theorem]{Condition}
\newtheorem{conjecture}[theorem]{Conjecture}
\newtheorem{corollary}[theorem]{Corollary}
\newtheorem{criterion}[theorem]{Criterion}
\newtheorem{definition}[theorem]{Definition}
\newtheorem{example}[theorem]{Example}
\newtheorem{exercise}[theorem]{Exercise}
\newtheorem{lemma}[theorem]{Lemma}
\newtheorem{notation}[theorem]{Notation}
\newtheorem{problem}[theorem]{Problem}
\newtheorem{proposition}[theorem]{Proposition}
\newtheorem{remark}[theorem]{Remark}
\newtheorem{solution}[theorem]{Solution}
\newtheorem{summary}[theorem]{Summary}
\newenvironment{proof}[1][Proof]{\noindent\textbf{#1.} }{\ \rule{0.5em}{0.5em}}
\input{../../tcilatex}
\DeclareMathAccent{\wtilde}{\mathord}{largesymbols}{"65}
\pagestyle{fancy}
\fancyfoot[C]{\thepage}


\begin{document}


\begin{equation*}
\mathbf{X}^{\dagger }\mathbf{X}=\left[ 
\begin{array}{cccccccccccc}
12 & 4 & 4 & 4 & 6 & 6 & 2 & 2 & 2 & 2 & 2 & 2 \\ 
4 & 4 & 0 & 0 & 2 & 2 & 2 & 2 & 0 & 0 & 0 & 0 \\ 
4 & 0 & 4 & 0 & 2 & 2 & 0 & 0 & 2 & 2 & 0 & 0 \\ 
4 & 0 & 0 & 4 & 2 & 2 & 0 & 0 & 0 & 0 & 2 & 2 \\ 
6 & 2 & 2 & 2 & 6 & 0 & 2 & 0 & 2 & 0 & 2 & 0 \\ 
6 & 2 & 2 & 2 & 0 & 6 & 0 & 2 & 0 & 2 & 0 & 2 \\ 
2 & 2 &  &  & 2 & 0 & 2 &  &  &  &  & 0 \\ 
2 & 2 &  &  & 0 & 2 &  & 2 &  &  &  &  \\ 
2 &  & 2 &  & 2 & 0 &  &  & 2 &  &  &  \\ 
2 &  & 2 &  & 0 & 2 &  &  &  & 2 &  &  \\ 
2 &  &  & 2 & 2 & 0 &  &  &  &  & 2 &  \\ 
2 &  &  & 2 & 0 & 2 & 0 &  &  &  &  & 2%
\end{array}%
\right] \quad \mathbf{X}^{\dagger }\mathbf{Y}=\left[ 
\begin{array}{c}
y_{\cdot \cdot \cdot } \\ 
y_{1\cdot \cdot } \\ 
y_{2\cdot \cdot } \\ 
y_{3\cdot \cdot } \\ 
y_{\cdot 1\cdot } \\ 
y_{\cdot 2\cdot } \\ 
y_{11\cdot } \\ 
y_{12\cdot } \\ 
y_{21\cdot } \\ 
y_{22\cdot } \\ 
y_{31\cdot } \\ 
y_{32\cdot }%
\end{array}%
\right] 
\end{equation*}

\bigskip 

the normal equations can be expressed as%
\begin{eqnarray*}
\overset{\text{abn}}{12}\hat{\mu}+\overset{\text{bn}}{4}\sum\limits_{i=1}^{3}%
\hat{\alpha}_{i}+\overset{\text{an}}{6}\sum\limits_{j=1}^{2}\hat{\beta}_{j}+%
\overset{\text{n}}{2}\sum\limits_{i=1}^{3}\sum\limits_{j=1}^{2}\hat{\gamma}%
_{ij} &=&y_{\cdot \cdot \cdot } \\
\overset{\text{bn}}{4}\hat{\mu}+\overset{\text{bn}}{4}\hat{\alpha}_{i}+%
\overset{\text{n}}{2}\sum\limits_{j=1}^{2}\hat{\beta}_{j}+\overset{\text{n}}{%
2}\sum\limits_{j=1}^{2}\hat{\gamma}_{ij} &=&y_{i\cdot \cdot }\quad i=1,2,3 \\
\overset{\text{an}}{6}\hat{\mu}+\overset{\text{n}}{2}\sum\limits_{i=1}^{2}%
\hat{\alpha}_{i}+\overset{\text{an}}{6}\hat{\beta}_{j}+\overset{\text{n}}{2}%
\sum\limits_{i=1}^{3}\hat{\gamma}_{ij} &=&y_{\cdot j\cdot }\quad j=1,2 \\
\overset{\text{n}}{2}\hat{\mu}+\overset{\text{n}}{2}\hat{\alpha}_{i}+\overset%
{\text{n}}{2}\hat{\beta}_{j}+\overset{\text{n}}{2}\hat{\gamma}_{ij}
&=&y_{ij\cdot }\quad 
\begin{tabular}{l}
$i=1,2,3$ \\ 
$j=1,2$%
\end{tabular}%
\end{eqnarray*}

Using the side conditions $\sum \hat{\alpha}_{i}=0$, $\sum\limits_{j=1}\hat{%
\beta}_{j}=0$, $\sum\limits_{i=1}\hat{\gamma}_{ij}=0$, $\sum\limits_{j}\hat{%
\gamma}_{ij}=0$, the solution to normal Equations is given by%
\begin{eqnarray*}
\hat{\mu} &=&\frac{y_{\cdot \cdot \cdot }}{12}=\bar{y}_{\cdot \cdot \cdot }
\\
\hat{\alpha}_{i} &=&\frac{y_{i\cdot \cdot }}{4}-\hat{\mu}=\bar{y}_{i\cdot
\cdot }-\bar{y}_{\cdot \cdot \cdot } \\
\hat{\beta}_{j} &=&\frac{y_{\cdot j\cdot }}{6}-\hat{\mu}=\bar{y}_{\cdot
j\cdot }-\bar{y}_{\cdot \cdot \cdot } \\
\hat{\gamma}_{ij} &=&\frac{y_{ij\cdot }}{2}-\hat{\alpha}_{i}-\hat{\beta}_{j}-%
\hat{\mu}=\bar{y}_{ij\cdot }-\bar{y}_{i\cdot \cdot }-\bar{y}_{\cdot j\cdot }+%
\bar{y}_{\cdot \cdot \cdot }
\end{eqnarray*}%
\begin{eqnarray*}
S^{2} &=&\frac{\text{SSE}}{ab\left( n-1\right) }=\frac{\mathbf{Y}^{\dagger
}\left( I-P_{\mathbf{X}}\right) \mathbf{Y}}{ab\left( n-1\right) }=\frac{%
\mathbf{Y}^{\dagger }\left( I-\mathbf{X}\left( \mathbf{X}^{\dagger }\mathbf{X%
}\right) ^{-}\mathbf{X}^{\dagger }\right) \mathbf{Y}}{ab\left( n-1\right) }
\\
&=&\frac{\mathbf{Y}^{\dagger }\mathbf{Y}-\mathbf{\hat{\beta}}^{\dagger }%
\mathbf{X}^{\dagger }\mathbf{Y}}{ab\left( n-1\right) }
\end{eqnarray*}%
is unbiased estimator of $\sigma ^{2}$.

\begin{eqnarray*}
&&\mathbf{\hat{\beta}}^{\dagger }\mathbf{X}^{\dagger }\mathbf{Y} \\
&=&\left[ 
\begin{array}{ccccccc}
\bar{y}_{\cdot \cdot \cdot } & \bar{y}_{i\cdot \cdot }-\bar{y}_{\cdot \cdot
\cdot } & \cdots & \bar{y}_{\cdot j\cdot }-\bar{y}_{\cdot \cdot \cdot } & 
\cdots & \bar{y}_{11\cdot }-\bar{y}_{1\cdot \cdot }-\bar{y}_{\cdot 1\cdot }+%
\bar{y}_{\cdot \cdot \cdot } & \cdots%
\end{array}%
\right] \left[ 
\begin{array}{c}
y_{\cdot \cdot \cdot } \\ 
y_{1\cdot \cdot } \\ 
\vdots \\ 
y_{\cdot 1\cdot } \\ 
\vdots \\ 
y_{11\cdot } \\ 
\vdots \\ 
y_{ab\cdot }%
\end{array}%
\right]
\end{eqnarray*}%
\begin{eqnarray*}
&=&\bar{y}_{\cdot \cdot \cdot }y_{\cdot \cdot \cdot }+y_{1\cdot \cdot
}\left( \bar{y}_{1\cdot \cdot }-\bar{y}_{\cdot \cdot \cdot }\right) +\cdots
+y_{a\cdot \cdot }\left( \bar{y}_{a\cdot \cdot }-\bar{y}_{\cdot \cdot \cdot
}\right) \\
&&+y_{\cdot 1\cdot }\left( \bar{y}_{\cdot 1\cdot }-\bar{y}_{\cdot \cdot
\cdot }\right) +\cdots +y_{\cdot b\cdot }\left( \bar{y}_{\cdot b\cdot }-\bar{%
y}_{\cdot \cdot \cdot }\right) \\
&&+y_{11\cdot }\left( \bar{y}_{11\cdot }-\bar{y}_{\cdot \cdot \cdot }\right)
+\cdots +y_{ab\cdot }\left( \bar{y}_{ab\cdot }-\bar{y}_{\cdot \cdot \cdot
}\right) \\
&=&\sum\limits_{i=1}^{a}\sum_{j=1}^{b}\bar{y}_{ij\cdot }\underset{n\bar{y}%
_{ij\cdot }}{\underbrace{y_{ij\cdot }}}=n\sum\limits_{i=1}^{a}\sum_{j=1}^{b}%
\bar{y}_{ij\cdot }^{2}=\sum\limits_{i=1}^{a}\sum_{j=1}^{b}\frac{y_{ij\cdot
}^{2}}{n}
\end{eqnarray*}%
\begin{equation*}
\mathbf{Y}^{\dagger }\mathbf{Y}-\mathbf{\hat{\beta}}^{\dagger }\mathbf{X}%
^{\dagger }\mathbf{Y}=\sum\limits_{i}\sum\limits_{j}\sum\limits_{k}y_{ijk}-n%
\sum\limits_{i}\sum\limits_{j}\bar{y}_{ij\cdot
}^{2}=\sum\limits_{i}\sum\limits_{j}\sum\limits_{k}\left( y_{ijk}-\bar{y}%
_{ij\cdot }\right) ^{2}
\end{equation*}%
\begin{equation*}
\therefore \text{SSE}=\sum\limits_{ijk}\left( y_{ijk}-\bar{y}_{ij\cdot
}\right) ^{2}
\end{equation*}

\bigskip

\subsubsection{Testing Hypotheses}

\paragraph{Full-Reduced-Model Approach (main effects $H_{0}:\protect\alpha %
_{1}=\cdots =\protect\alpha _{a}$)}

\begin{equation*}
\begin{tabular}{l}
the full model is $y_{ijk}=\mu +\alpha _{i}+\beta _{j}+\gamma
_{ij}+\varepsilon _{ijk}$ \\ 
the reduced model is $y_{ijk}=\mu +\beta _{j}+\gamma _{ij}+\varepsilon
_{ijk} $%
\end{tabular}%
\end{equation*}%
\begin{eqnarray*}
\mathbf{\hat{\beta}}^{\dagger }\mathbf{X}^{\dagger }\mathbf{Y} &=&\bar{y}%
_{\cdot \cdot \cdot }y_{\cdot \cdot \cdot }+y_{\cdot 1\cdot }\left( \bar{y}%
_{\cdot 1\cdot }-\bar{y}_{\cdot \cdot \cdot }\right) +\cdots +y_{\cdot
b\cdot }\left( \bar{y}_{\cdot b\cdot }-\bar{y}_{\cdot \cdot \cdot }\right) \\
&&+y_{11\cdot }\left( \bar{y}_{11\cdot }-\bar{y}_{\cdot \cdot \cdot }\right)
+\cdots +y_{ab\cdot }\left( \bar{y}_{ab\cdot }-\bar{y}_{\cdot \cdot \cdot
}\right)
\end{eqnarray*}%
\begin{eqnarray*}
&\therefore &\text{SSR}=\mathbf{\hat{\beta}}^{\dagger }\mathbf{X}^{\dagger }%
\mathbf{Y}-\mathbf{\hat{\beta}}_{1}^{\dagger }\mathbf{X}_{1}^{\dagger }%
\mathbf{Y=}y_{1\cdot \cdot }\left( \bar{y}_{1\cdot \cdot }-\bar{y}_{\cdot
\cdot \cdot }\right) +\cdots +y_{a\cdot \cdot }\left( \bar{y}_{a\cdot \cdot
}-\bar{y}_{\cdot \cdot \cdot }\right) \\
&=&\sum\limits_{i=1}^{n}\frac{y_{i\cdot \cdot }^{2}}{bn}-\bar{y}_{\cdot
\cdot \cdot }\sum\limits_{i=1}^{a}\bar{y}_{i\cdot \cdot } \\
&=&\sum\limits_{i=1}^{n}\frac{y_{i\cdot \cdot }^{2}}{bn}-\frac{y_{\cdot
\cdot \cdot }^{2}}{abn}=bn\sum\limits_{i=1}^{a}\left( y_{i\cdot \cdot }-\bar{%
y}_{\cdot \cdot \cdot }\right) ^{2}
\end{eqnarray*}

$H_{0}:\beta _{1}=\cdots =\beta _{b}$%
\begin{equation*}
\text{SSR}=\sum\limits_{j=1}^{b}\frac{y_{\cdot j\cdot }^{2}}{an}-\frac{%
y_{\cdot \cdot \cdot }^{2}}{abn}
\end{equation*}

$H_{0}:\gamma _{ij}=0$%
\begin{equation*}
\text{SSR}=\sum\limits_{i=1}^{a}\sum\limits_{j=1}^{b}\frac{y_{ij\cdot }^{2}}{%
n}-\sum\limits_{i=1}^{a}\frac{y_{i\cdot \cdot }^{2}}{bn}-\sum%
\limits_{j=1}^{b}\frac{y_{\cdot j\cdot }^{2}}{an}+\frac{y_{\cdot \cdot \cdot
}^{2}}{abn}
\end{equation*}

\bigskip

\begin{equation*}
\begin{tabular}{lllll}
S.V. & df & \c{S}\c{S} & M.S. & E(M.S.) \\ \hline
Factor A & \multicolumn{1}{|l}{$a-1$} & $\sum\limits_{i=1}^{a}\frac{%
y_{i\cdot \cdot }^{2}}{bn}-\frac{y_{\cdot \cdot \cdot }^{2}}{abn}$ & $\frac{%
\text{SSA}}{a-1}$ & $\sigma ^{2}+bn\frac{\sum \alpha _{i}^{2}}{a-1}$ \\ 
Factor B & \multicolumn{1}{|l}{$b-1$} & $\sum\limits_{j=1}^{b}\frac{y_{\cdot
j\cdot }^{2}}{an}-\frac{y_{\cdot \cdot \cdot }^{2}}{abn}$ & $\frac{\text{SSB}%
}{b-1}$ & $\sigma ^{2}+an\frac{\sum \beta _{j}^{2}}{b-1}$ \\ 
Intersection & \multicolumn{1}{|l}{$%
\begin{array}{c}
\left( a-1\right) \times \\ 
\left( b-1\right)%
\end{array}%
$} & $%
\begin{array}{c}
\sum\limits_{i=1}^{a}\sum\limits_{j=1}^{b}\frac{y_{ij\cdot }^{2}}{n}%
-\sum\limits_{i=1}^{a}\frac{y_{i\cdot \cdot }^{2}}{bn} \\ 
-\sum\limits_{j=1}^{b}\frac{y_{\cdot j\cdot }^{2}}{an}+\frac{y_{\cdot \cdot
\cdot }^{2}}{abn}%
\end{array}%
$ & $\frac{\text{SSAB}}{\left( a-1\right) \left( b-1\right) }$ & $%
\begin{array}{c}
\sigma ^{2}+ \\ 
n\sum\limits_{i}\sum\limits_{j}\frac{\gamma _{ij}^{2}}{\left( a-1\right)
\left( b-1\right) }%
\end{array}%
$ \\ 
Error & \multicolumn{1}{|l}{$ab\left( n-1\right) $} & $%
\begin{array}{c}
\sum\limits_{i}\sum\limits_{j}\sum\limits_{k}y_{ijk}^{2}-\sum\limits_{i}\sum%
\limits_{j}\frac{y_{ij\cdot }^{2}}{n} \\ 
\left( \sum\limits_{i}\sum\limits_{j}\sum\limits_{k}\left( y_{ijk}-\bar{y}%
_{ij\cdot }\right) ^{2}\right)%
\end{array}%
$ & $\frac{\text{SSE}}{ab\left( n-1\right) }$ & $\sigma ^{2}$ \\ 
Total & \multicolumn{1}{|l}{$abn-1$} & $\sum\limits_{i}\sum\limits_{j}\sum%
\limits_{k}y_{ijk}^{2}-\frac{y_{\cdot \cdot \cdot }^{2}}{abn}$ &  & 
\end{tabular}%
\end{equation*}

\bigskip

\begin{equation*}
E\left( \text{MSA}\right) =E\left( \frac{\text{SSA}}{a-1}\right) =\frac{1}{%
a-1}E\left( \sum\limits_{i=1}^{a}\frac{y_{i\cdot \cdot }^{2}}{bn}-\frac{%
y_{\cdot \cdot \cdot }^{2}}{abn}\right)
\end{equation*}

\begin{eqnarray*}
E\left( y_{\cdot \cdot \cdot }^{2}\right) &=&E\left[ \left(
\sum\limits_{i}\sum\limits_{j}\sum\limits_{k}y_{ijk}\right) ^{2}\right] \\
&=&E\left[ \left( \sum \sum \sum \left( \mu +\alpha _{i}+\beta _{j}+\gamma
_{ij}+\varepsilon _{ijk}\right) \right) ^{2}\right] \\
&=&E\left[ \left( abn\mu +\beta n\sum \alpha _{i}+an\sum \beta _{j}+n\sum
\sum \gamma _{ij}+\sum\limits_{ijk}\varepsilon _{ijk}\right) ^{2}\right] \\
&=&E\left[ a^{2}b^{2}n^{2}\mu ^{2}+2abn\mu \left(
\sum\limits_{ijk}\varepsilon _{ijk}\right) +\left(
\sum\limits_{ijk}\varepsilon _{ijk}\right) ^{2}\right] \\
&=&a^{2}b^{2}n^{2}\mu ^{2}+2abn\mu \left( \sum\limits_{ijk}\varepsilon
_{ijk}\right) +E\left( \sum\limits_{ijk}\varepsilon _{ijk}^{2}\right)
+E\left( \sum\limits_{ijk=rst}\varepsilon _{ijk}\varepsilon _{rst}\right) \\
&=&a^{2}b^{2}n^{2}\mu ^{2}+abn\sigma ^{2}
\end{eqnarray*}%
\begin{equation*}
E\left( \varepsilon _{ijk}\right) =0\quad E\left( \varepsilon
_{ijk}^{2}\right) =\sigma ^{2}\quad E\left( \varepsilon _{ijk}\varepsilon
_{rst}\right) =0
\end{equation*}

\bigskip

\begin{eqnarray*}
E\left( \sum\limits_{i=1}^{a}y_{i\cdot \cdot }^{2}\right) &=&E\left[
\sum\limits_{i=1}^{a}\left(
\sum\limits_{j=1}^{b}\sum\limits_{k=1}^{n}y_{ijk}\right) ^{2}\right] \\
&=&\cdots \\
&=&a^{2}b^{2}n^{2}\mu ^{2}+b^{2}n^{2}\sum_{i=1}^{a}\alpha _{i}^{2}+abn\sigma
^{2}
\end{eqnarray*}

\begin{eqnarray*}
E\left( \text{MSA}\right) &=&\frac{1}{a-1}\left[ \frac{a^{2}b^{2}n^{2}\mu
^{2}+b^{2}n^{2}\sum_{i=1}^{a}\alpha _{i}^{2}+abn\sigma ^{2}}{bn}-\frac{%
a^{2}b^{2}n^{2}\mu ^{2}+abn\sigma ^{2}}{abn}\right] \\
&=&\frac{1}{a-1}\left[ abn\mu ^{2}+bn\sum \alpha _{i}^{2}+a\sigma
^{2}-abn\mu ^{2}-\sigma ^{2}\right] \\
&=&\frac{1}{a-1}\left[ \sigma ^{2}\left( a-1\right) +bn\sum \alpha _{i}^{2}%
\right] =\sigma ^{2}+\frac{bn\sum \alpha _{i}^{2}}{a-1}
\end{eqnarray*}

\bigskip

\bigskip

\subsubsection{General Linear Hypothesis}

Consider $\mathbf{\beta }^{\dagger }=\left[ 
\begin{array}{cccccccccccc}
\mu & \alpha _{1} & \alpha _{2} & \alpha _{3} & \beta _{1} & \beta _{2} & 
\gamma _{11} & \gamma _{12} & \gamma _{21} & \gamma _{22} & \gamma _{31} & 
\gamma _{32}%
\end{array}%
\right] $ and the hypothesis $H_{0}:\alpha _{1}=\alpha _{2}=\alpha _{3}$

\bigskip

the hypothesis can be expressed as%
\begin{equation*}
H_{0}:\left[ 
\begin{array}{c}
\alpha _{1}+\frac{1}{2}\gamma _{11}+\frac{1}{2}\gamma _{12}-\alpha _{3}-%
\frac{1}{2}\gamma _{31}-\frac{1}{2}\gamma _{22} \\ 
\alpha _{2}+\frac{1}{2}\gamma _{21}+\frac{1}{2}\gamma _{22}-\alpha _{3}-%
\frac{1}{2}\gamma _{31}-\frac{1}{2}\gamma _{32}%
\end{array}%
\right] =\left[ 
\begin{array}{c}
0 \\ 
0%
\end{array}%
\right]
\end{equation*}%
\begin{equation*}
\Rightarrow H_{0}:\mathbf{C\beta =0},\text{ where}
\end{equation*}%
\begin{equation*}
\mathbf{0}=\left[ 
\begin{array}{cccccccccccc}
0 & 1 & 0 & -1 & 0 & 0 & \frac{1}{2} & \frac{1}{2} & 0 & 0 & -\frac{1}{2} & -%
\frac{1}{2} \\ 
0 & 0 & 1 & -1 & 0 & 0 & 0 & 0 & \frac{1}{2} & \frac{1}{2} & -\frac{1}{2} & -%
\frac{1}{2}%
\end{array}%
\right]
\end{equation*}

note: the matrix $\mathbf{C}$ is not unique

\bigskip

\begin{eqnarray*}
\text{SSH} &=&\left( \mathbf{C\hat{\beta}}\right) ^{\dagger }\left[ \mathbf{C%
}\left( \mathbf{X}^{\dagger }\mathbf{X}\right) ^{-1}\mathbf{C}^{\dagger }%
\right] ^{-1}\left( \mathbf{C\hat{\beta}}\right) \\
&=&\mathbf{Y}^{\dagger }\underset{\left( \ast \right) }{\underbrace{\mathbf{X%
}\left( \mathbf{X}^{\dagger }\mathbf{X}\right) ^{-1}\mathbf{C}^{\dagger }%
\left[ \mathbf{C}\left( \mathbf{X}^{\dagger }\mathbf{X}\right) ^{-1}\mathbf{C%
}^{\dagger }\right] ^{-1}\mathbf{C\left( \mathbf{X}^{\dagger }\mathbf{X}%
\right) ^{-1}\mathbf{X}^{\dagger }}}}\mathbf{Y}
\end{eqnarray*}%
\begin{equation*}
\because \left( \mathbf{X}^{\dagger }\mathbf{X}\right) ^{-1}=\frac{1}{2}%
\left[ 
\begin{array}{cc}
\mathbf{0}_{6\times 6} & \mathbf{0}_{6\times 6} \\ 
\mathbf{0}_{6\times 6} & I_{6}%
\end{array}%
\right] \text{ and }\mathbf{C}\left( \mathbf{X}^{\dagger }\mathbf{X}\right)
^{-1}\mathbf{C}^{\dagger }=\frac{1}{4}\left[ 
\begin{array}{cc}
2 & 1 \\ 
1 & 2%
\end{array}%
\right]
\end{equation*}%
\begin{equation*}
\therefore \left[ \mathbf{C}\left( \mathbf{X}^{\dagger }\mathbf{X}\right)
^{-1}\mathbf{C}^{\dagger }\right] ^{-1}=\frac{4}{3}\left[ 
\begin{array}{cc}
2 & -1 \\ 
-1 & 2%
\end{array}%
\right]
\end{equation*}%
\begin{equation*}
\mathbf{C}\left( \mathbf{X}^{\dagger }\mathbf{X}\right) ^{-1}\mathbf{X}%
^{\dagger }=\left[ 
\begin{array}{cccccccccccc}
1 & 1 & 1 & 1 & 0 & 0 & 0 & 0 & -1 & -1 & -1 & -1 \\ 
0 & 0 & 0 & 0 & 1 & 1 & 1 & 1 & -1 & -1 & -1 & -1%
\end{array}%
\right]
\end{equation*}

\begin{equation*}
\left( \ast \right) \Rightarrow \frac{1}{12}\left[ 
\begin{array}{ccc}
2J_{4} & -J & -J \\ 
-J & 2J & -J \\ 
-J & -J & 2J%
\end{array}%
\right] =\frac{1}{12}\left[ 
\begin{array}{ccc}
3J & 0 & 0 \\ 
0 & 3J & 0 \\ 
0 & 0 & 3J%
\end{array}%
\right] -\frac{1}{12}\left[ 
\begin{array}{ccc}
J & J & J \\ 
J & J & J \\ 
J & J & J%
\end{array}%
\right] =\mathbf{A}
\end{equation*}

\begin{eqnarray*}
&\therefore &\text{SSA}=\mathbf{Y}^{\dagger }\mathbf{AY=}\frac{1}{12}\mathbf{%
Y}^{\dagger }\left[ 
\begin{array}{ccc}
3J_{4} & 0 & 0 \\ 
0 & 3J & 0 \\ 
0 & 0 & 3J%
\end{array}%
\right] \mathbf{Y}-\frac{1}{12}\mathbf{Y}^{\dagger }\left[ 
\begin{array}{ccc}
J & J & J \\ 
J & J & J \\ 
J & J & J%
\end{array}%
\right] \mathbf{Y} \\
&=&\frac{3}{12}\sum\limits_{i=1}^{3}\mathbf{y}_{i}^{\dagger }J\mathbf{y}_{i}-%
\frac{1}{12}\mathbf{Y}^{\dagger }J_{12}\mathbf{Y,}\text{ where }\mathbf{Y}%
^{\dagger }=\left[ 
\begin{array}{ccc}
\mathbf{y}_{1}^{\dagger } & \mathbf{y}_{2}^{\dagger } & \mathbf{y}%
_{3}^{\dagger }%
\end{array}%
\right] \\
&=&\frac{1}{4}\sum\limits_{i=1}^{3}\mathbf{y}_{i}^{\dagger }\mathbf{1}_{4}%
\mathbf{1}^{\dagger }\mathbf{y}_{i}-\frac{1}{12}\mathbf{Y}^{\dagger }\mathbf{%
1}_{12}\mathbf{1}_{12}^{\dagger }\mathbf{Y} \\
&=&\sum\limits_{i=1}^{3}\frac{y_{i\cdot }^{2}}{4}-\frac{y_{\cdot \cdot \cdot
}^{2}}{12}
\end{eqnarray*}

\end{document}
